progs/verif_global.v
@@ -30,9 +30,212 @@ forward.  (* x = g; *)
 forward.  (* return x; *)
 Qed.
 
+Ltac start_function1 :=
+ match goal with |- semax_body _ _ ?F ?spec =>
+   let D := constr:(type_of_function F) in 
+   let S := constr:(type_of_funspec (snd spec)) in
+   let D := eval hnf in D in let D := eval simpl in D in 
+   let S := eval hnf in S in let S := eval simpl in S in 
+   tryif (unify D S) then idtac else
+   tryif function_types_compatible D S 
+   then idtac "Warning: the function-body parameter/return types are not identical to the funspec types, although they are compatible:
+Function body:" D "
+Function spec:" S
+   else
+   (fail "Function signature (param types, return type) from function-body does not match function signature from funspec
+Function body: " D "
+Function spec: " S)
+ end;
+ match goal with |- semax_body ?V ?G ?F ?spec =>
+    let s := fresh "spec" in
+    pose (s:=spec); hnf in s;
+    match goal with
+    | s :=  (DECLARE _ WITH _: globals
+               PRE  [] main_pre _ nil _
+               POST [ tint ] _) |- _ => idtac
+    | s := ?spec' |- _ => check_canonical_funspec spec'
+   end;
+   change (semax_body V G F s); subst s
+ end;
+ let DependedTypeList := fresh "DependedTypeList" in
+ match goal with |- semax_body _ _ _ (pair _ (NDmk_funspec _ _ _ ?Pre _)) =>
+   match Pre with
+   | (fun x => match _ with (a,b) => _ end) => intros Espec DependedTypeList [a b]
+   | (fun i => _) => intros Espec DependedTypeList i
+   end;
+   simpl fn_body; simpl fn_params; simpl fn_return
+ end;
+ simpl functors.MixVariantFunctor._functor in *;
+ simpl rmaps.dependent_type_functor_rec;
+ clear DependedTypeList;
+ repeat match goal with |- @semax _ _ _ (match ?p with (a,b) => _ end * _) _ _ =>
+             destruct p as [a b]
+           end;
+ simplify_func_tycontext;
+ repeat match goal with
+ | |- context [Sloop (Ssequence (Sifthenelse ?e Sskip Sbreak) ?s) Sskip] =>
+       fold (Swhile e s)
+ | |- context [Ssequence ?s1 (Sloop (Ssequence (Sifthenelse ?e Sskip Sbreak) ?s2) ?s3) ] =>
+      match s3 with
+      | Sset ?i _ => match s1 with Sset ?i' _ => unify i i' | Sskip => idtac end
+      end;
+      fold (Sfor s1 e s2 s3)
+ end.
+
+
+Ltac process_one_globvar :=
+ first
+  [ simple eapply process_globvar_space;
+    [simpl; reflexivity | reflexivity | reflexivity | reflexivity | reflexivity | reflexivity | simpl; computable | ]
+  | simple eapply process_globvar';
+      [reflexivity | reflexivity | reflexivity | reflexivity | reflexivity | reflexivity
+      | reflexivity | compute; congruence | ]
+  | fail; (* admitted *)
+    simple eapply process_globvar_array;
+      [reflexivity | reflexivity | reflexivity | reflexivity | reflexivity | apply Coq.Init.Logic.I
+      | compute; clear; congruence
+      | repeat eapply map_instantiate; symmetry; apply map_nil
+      | compute; split; clear; congruence |  ]
+  | fail; (* admitted *)
+    simple eapply process_globvar_star';
+        [reflexivity | reflexivity | reflexivity
+        | reflexivity | compute; split; clear; congruence
+       | simpl gvar_info; simpl gvar_readonly; simpl readonly2share;
+         change (Share.lub extern_retainer Tsh) with Ews
+         ]
+  ];
+  change (Share.lub extern_retainer _) with Ews;
+  change (Share.lub extern_retainer _) with Ers;
+  change (Vint oo _) with (Vint oo id);
+  fold_types;
+  rewrite ?Combinators.compose_id_right.
+
 Lemma body_main:  semax_body Vprog Gprog f_main main_spec.
 Proof.
-start_function.
+start_function1.
+ rewrite main_pre_start; unfold prog_vars, prog_vars'; simpl globvars2pred.
+process_one_globvar.
+process_one_globvar.
+
+Definition globvar2pred' (gv : globals) (i : ident) (v: globvar type) :=
+if gvar_volatile v
+then lift0 TT
+else
+ init_data_list2pred (gvar_init v) (readonly2share (gvar_readonly v))
+   (offset_val 0 (gv i)).
+
+Lemma one_globvar2pred: forall gv i v vl,
+  gvar_volatile v = false ->
+  globvars2pred gv ((i,v)::vl) = 
+    (local (`(eq gv) globals_of_env) &&
+    (init_data_list2pred (gvar_init v) (readonly2share (gvar_readonly v))
+              (offset_val 0 (gv i))))
+     * globvars2pred gv vl.
+Proof.
+intros.
+unfold globvars2pred; fold globvars2pred.
+extensionality rho.
+unfold_lift.
+unfold local, lift1, lift2.
+simpl.
+unfold globvar2pred at 1.
+simpl. rewrite H.
+apply pred_ext; normalize.
+rewrite prop_true_andp by auto.
+rewrite !offset_zero_globals_of_env; auto.
+rewrite !offset_zero_globals_of_env; auto.
+Qed.
+
+rewrite one_globvar2pred by reflexivity.
+match goal with |- semax ?D (?P1 * (?P2 * ?P3) * ?P4) ?C ?Q =>
+   pose (CTX x := semax D (P1 * (x * P3) * P4) C Q);
+   change (CTX P2)
+end.
+clearbody CTX.
+
+set (sh :=  readonly2share (gvar_readonly _)).
+simpl gvar_init.
+
+change (init_data_list2pred (?A::?B) ?sh ?v) 
+    with (init_data2pred A (Share.lub extern_retainer sh) v * init_data_list2pred B sh (offset_val (init_data_size A) v));
+cbv beta;
+rewrite ?offset_offset_val;
+simpl Z.add.
+
+Lemma init_data2pred_rejigger:
+  forall {cs : compspecs} (Delta : tycontext) (idata : init_data) 
+    (rho : environ) (sh : Share.t) (b : block) (ofs : Z) (v : val),
+  tc_environ Delta rho ->
+  v = Vptr b (Ptrofs.repr 0) ->
+  readable_share sh ->
+  init_data2pred idata sh (offset_val ofs v) rho
+  |-- init_data2pred' Delta (globals_of_env rho) idata sh (offset_val ofs v) rho.
+
+
+Search init_data2pred.
+unfold init_data2pred.
+
+
+change (init_data_list2pred (?A::?B) ?sh ?v) 
+    with (init_data2pred A (Share.lub extern_retainer sh) v * init_data_list2pred B sh (offset_val (init_data_size A) v));
+simpl init_data_size;
+rewrite ?offset_offset_val;
+simpl Z.add.
+
+change (init_data_list2pred (?A::?B) ?sh ?v) 
+    with (init_data2pred A (Share.lub extern_retainer sh) v * init_data_list2pred B sh (offset_val (init_data_size A) v));
+simpl init_data_size;
+rewrite offset_offset_val;
+simpl Z.add.
+
+match goal 
+
+unfold gvar_init.
+unfold init_data_list2pred.
+
+; cbv beta zeta.
+simpl.
+unfold globals_of_env.
+unfold gvar_volatile; cbv iota. simpl fst; simpl snd.
+
+
+
+simpl gvar_init.
+
+
+
+match goal with |- context [initdatalist2pred (?A::?B)] =>
+  change (initdatalist2pred (?A::?B) ?sh ?v) with (initdat2pred A 
+simpl.
+Locate mapsto_.
+unfold init_data
+simpl.
+
+
+unfold init_data_list2pred.
+
+
+
+normalize.
+Definition globvars2pred  (gv: globals)  (vl: list (ident * globvar type)) : environ->mpred :=
+  (lift2 andp) (fun rho => prop (gv = globals_of_env rho))
+  (fold_right sepcon emp (map (globvar2pred gv) vl)).
+
+Search globvars2pred.
+
+simple eapply process_globvar_array;
+      [reflexivity | reflexivity | reflexivity | reflexivity | reflexivity | apply Coq.Init.Logic.I
+      | compute; clear; congruence
+      | repeat eapply map_instantiate; symmetry; apply map_nil
+      | compute; split; clear; congruence |  ].
+
+process_one_globvar.
+
+
+process_idstar.
+
+
+
 rewrite data_at_tuint_tint.
 forward_call gv.
 forward.
