veric/mapsto_memory_block.v
@@ -389,7 +389,7 @@ Definition mapsto_zeros (n: Z) (sh: share) (a: val) : mpred :=
   | Vptr b z => 
     !! (0 <= Ptrofs.unsigned z  /\ n + Ptrofs.unsigned z < Ptrofs.modulus)%Z &&
     address_mapsto_zeros sh (nat_of_Z n) (b, Ptrofs.unsigned z)
-  | _ => TT
+  | _ => FF
   end.
 
 Fixpoint memory_block' (sh: share) (n: nat) (b: block) (i: Z) : mpred :=
@@ -907,16 +907,16 @@ Proof.
   omega.
 Qed.
 
-Lemma mapsto_zeros_memory_block: forall sh n b ofs,
-(*  n < Ptrofs.modulus ->
-  Ptrofs.unsigned ofs+n < Ptrofs.modulus ->
-*)  readable_share sh ->
-  mapsto_zeros n sh (Vptr b ofs) |--
-  memory_block sh n (Vptr b ofs).
+Lemma mapsto_zeros_memory_block: forall sh n p,
+  readable_share sh ->
+  mapsto_zeros n sh p |--
+  memory_block sh n p.
 Proof.
+  intros.
   unfold mapsto_zeros.
+  destruct p; try solve [intros ? ?; contradiction].
+  rename i into ofs.
   intros. rename H into RS. pose proof I.
-(*  rename H0 into H'. rename H1 into RS. *)
   unfold memory_block.
   destruct (zlt n 0).   {
      rewrite nat_of_Z_neg by omega. simpl.
@@ -928,10 +928,6 @@ Proof.
  rewrite prop_true_andp by omega.
  assert (n <= Ptrofs.modulus) by omega. clear H H0. rename H1 into H'.
  assert (0 <= n <= Ptrofs.modulus) by omega. clear H2 g.
-(*  repeat rewrite Int.unsigned_repr by omega. 
-  apply andp_right.  
-  + intros ? _; auto. 
-  + *)
     rewrite <- (Z2Nat.id n) in H', H by omega.
     change nat_of_Z with Z.to_nat.
     forget (Z.to_nat n) as n'.
